---
{"dg-publish":true,"permalink":"/content/012/px-285-hamiltonian-mechanics-and-fluid-dynamics/term-2-fluid-dynamics/j-some-approximate-solutions/px-285-j7-surface-waves/","noteIcon":"1","created":"2025-08-27T13:15:24.277+01:00","updated":"2025-02-01T16:03:24.000+00:00"}
---

![PX285 - I3d - surface waves.png|500](/img/user/pics/PX285%20-%20I3d%20-%20surface%20waves.png)

- moving to the frame of reference of the wave so that bernoulli's principle is applicable
- from mass conservation:
$$\begin{gather}
u_{1} \left(h + \frac{\psi}{2}\right) = u_{2} \left(h - \frac{\psi}{2}\right) \\
\frac{\psi}{2} (u_{1}+ u_{2}) = h (u_{2}- u_{1}) \tag {1}
\end{gather}$$
- applying bernoulli's principle:
$$\begin{gather}
\rho g \left(h + \frac{\psi}{2}\right) + \rho \frac{u_{1}^{2}}{2} = \rho g\left(h - \frac{\psi}{2}\right) + \rho \frac{u_{2}^{2}}{2} \\
g \psi = \frac{u_{2}^{2}-u_{1}^{2}}{2} = \frac{(u_{2}-u_{1})(u_{2}+u_{1})}{2}
\end{gather}$$
- from equation $(1):$
$$\begin{gather}
g \psi = \frac{u_{2}^{2}-u_{1}^{2}}{2} = \frac{(u_{2}+u_{1})^{2}\psi}{4h} \\
gh = \left(\frac{u_{2}+u_{1}}{2}\right)^{2} = v_{phase}^{2}
\end{gather}$$
- therefore, the phase speed:
$$v_{phase} = \sqrt{gh}$$
