---
dg-publish: true
---

$$dI_{\lambda} = - \kappa_{\lambda}\rho I_{\lambda}\,dz + \epsilon_{\lambda}\rho \,dz$$
	where, $\kappa_{\lambda}= \kappa_{b-b} + \kappa_{b-f} + \kappa_{f-f} + \kappa_{H^{-}} + \kappa_{e-s}$
$$\frac{dI_{\lambda}}{\rho\kappa_{\lambda}\,dz} = -I_{\lambda} + \frac{\epsilon_{\lambda}}{\kappa_{\lambda}} = - I_{\lambda}+ S_\lambda$$
	where, $S_{\lambda}=$ the source function
$$- \frac{1}{\kappa_{\lambda}} \frac{dI_{\lambda}}{dz} = I_{\lambda}-S_{\lambda}$$
- consider the balance between $I_{\lambda}$ and $S_{\lambda}$
	- of $I_{\lambda} > S_{\lambda}: \frac{dI_{\lambda}}{dz}<0$ , so, $I_{\lambda}$ decreases with $z$
	- of $I_{\lambda} < S_{\lambda}: \frac{dI_{\lambda}}{dz}>0$ , so, $I_{\lambda}$ increases with $z$
- the beam intensity approaches the local value of the source function ($S_{la}$ may vary too quickly)
- in $\tau$-space, the radiative transfer equation is obtained: 
$$\frac{dI_{\lambda}}{d\tau_{\lambda}} = I_{\lambda}- S_{\lambda}$$
