---
{"dg-publish":true,"permalink":"/content/011/px-154-physics-foundations/px-154-f-waves/px-154-f1b-the-wave-function/","noteIcon":"1","created":"2024-11-25T10:50:32.000+00:00","updated":"2024-11-26T19:51:24.766+00:00"}
---

![Pasted image 20231115100442.png](/img/user/pics/Pasted%20image%2020231115100442.png)
- considering sinusoidal behaviour
- the wavelength is $\lambda$, so, at $x=\lambda$, we need $1$ complete cycle
- as $x$ goes from $0\to\lambda$, consider $\cos ax$ to go from $0\to 2\pi$ 
- take $\cos(\frac{2\pi}{\lambda}x)$: $\cos\left(\frac{2\pi}{\lambda}x\right)= 1$ at $2n\pi$, so, when $x = \lambda, \; 2\lambda, \; 3\lambda, \; etc$
- take 
$$\frac{2\pi}{\lambda} = k $$
			where $k=$ *wave number* with units $rad \, m^{-1}$ or $m^{-1}$
	- we have, $\cos(kx)$
- for time dependence at one x position
![Pasted image 20231115100521.png](/img/user/pics/Pasted%20image%2020231115100521.png)
- we can use $\cos(\frac{2\pi}{T}t)$:
	- $f = \frac{1}{T}$
	- we have $\cos(2\pi f \,t)$
	- and, we can write $\cos(\omega t)$
		- where, $\omega=$ angular frequency
- to put this together: ![Pasted image 20231115100607.png](/img/user/pics/Pasted%20image%2020231115100607.png)
- the waveform translates, but doesn't change shape: in the figure above, it translates from left $\to$ right
- we write: 
$$u(x,t) = A \cos(kx-\omega t)$$
- for right $\to$ left translation: $u(x,t)=A\cos(kx+\omega t)$
$$u(x,t) = A \cos(kx\pm\omega t)$$
		where, $A=$ amplitude, $k=$ wave number, $\omega =$ angular frequency 
- where, ${} -$ for right; $+$ for left travelling
